@prefix : <https://gcxgce.sharepoint.com/teams/1000944/#> .
@prefix dcterms: <http://purl.org/dc/terms/> .
@prefix gc: <https://www.canada.ca/#> .
@prefix lawslois: <https://laws-lois.justice.gc.ca/eng/acts/> .
@prefix owl: <http://www.w3.org/2002/07/owl#> .
@prefix rdfs: <http://www.w3.org/2000/01/rdf-schema#> .
@prefix schema: <https://schema.org/> .
@prefix schema1: <http://www.schema.org/> .
@prefix skos: <http://www.w3.org/2004/02/skos/core#> .
@prefix wiki: <https://en.wikipedia.org/wiki/> .
@prefix xsd: <http://www.w3.org/2001/XMLSchema#> .

:Policy a rdfs:Class ;
    rdfs:label "Public Policy" ;
    rdfs:comment "what governments choose to do, or not do" .

wiki:Fall_of_the_Berlin_Wall a schema:event ;
    rdfs:label "Fall of the Berlin Wall" ;
    schema:endDate "19891109T1901Z" ;
    schema:instrument :SovietUnionCollapse ;
    schema:location wiki:Berlin_Wall ;
    schema:startDate "19891109T1853Z" .

wiki:Government_Debt a skos:Concept ;
    rdfs:label "Government Debt",
        "National Debt" .

:Bloc_Quebecois a schema:PoliticalParty ;
    schema:foundingDate 1991 .

:ClerkPrivyCouncil a schema:organizationRole,
        gc:PublicServant ;
    :heads :PrivyCouncilOffice ;
    schema:additionalType gc:DeputyHead .

:Crown rdfs:label "Monarch"@en,
        "The Crown"@en ;
    schema:owns :CrownAsset ;
    gc:delegates :CrownAuthority ;
    gc:holds :CrownAuthority .

:Danger a :hasContext ;
    rdfs:label "Danger"@en ;
    rdfs:comment "e.g., rising threats, instability" .

:DataInfoManagement a schema:OrganizeAction ;
    rdfs:label "Data and Information Management" ;
    rdfs:comment "Information and data management is a discipline that directs and supports effective and efficient management of information and data in an organization, from planning and systems development to disposal and/or long-term preservation. In the Government of Canada, information and data are safeguarded as a public trust and managed as a strategic asset to maximize its value in the service of Canadians." ;
    schema:disambiguatingDescription "Integrated/unified management of both data and information. While they are not to be understood as mutually exclusive, their varying life cycles demand distinct practices." ;
    schema:isPartOf :EnterpriseArchitecture ;
    schema:subject :DataAndInfo ;
    schema:subjectOf "https://www.canada.ca/en/government/system/digital-government/digital-government-innovations/information-management.html" .

:DeliverPrograms a schema:OrganizeAction ;
    schema:isPartOf :DeliverResultsForCanadians .

:DeliverServices a schema:OrganizeAction ;
    schema:isPartOf :DeliverResultsForCanadians .

:Division a :hasContext ;
    rdfs:label "Division"@en ;
    rdfs:comment "e.g., political, social, or economic fragmentation" .

:GeopoliticalRisk a skos:Concept .

:Green_Canada a schema:PoliticalParty ;
    schema:foundingDate 1983 .

:Information a schema:Intangible ;
    rdfs:comment "Knowledge captured in any format, such as facts, events, things, processes, or ideas, that can be structured or unstructured, including concepts that within a certain context have particular meaning. Information includes data." ;
    skos:inScheme gc:ServiceDigitalDefs .

:JohnAMacdonald a schema:Person ;
    rdfs:label "John A. Macdonald" ;
    :holdsOffice :PrimeMinisterCanada1 ;
    schema:memberOf :Liberal_Conservative_Canada .

:Justin_Trudeau a schema:Person ;
    rdfs:label "Justin Trudeau" ;
    :holdsOffice :PrimeMinisterCanada23 ;
    schema:memberOf :Liberal_Canada .

:MandateLetter2025 a :MandateLetter ;
    rdfs:label "Mandate Letter (2025)"@en,
        "Lettre de mandat (2025)"@fr ;
    schema:about :CanadianContext2025,
        :GlobalContext2025,
        :Priorities2025 ;
    schema:author :Mark_Carney ;
    schema:dateCreated "2025-05-21" .

:New_Democratic_Canada a schema:PoliticalParty ;
    schema:foundingDate 1961 .

:Parti_Bleu a schema:PoliticalParty ;
    :succeededBy :Liberal_Conservative_Canada ;
    schema:dissolutionDate 1867 ;
    schema:foundingDate 1854 .

:Policy_Carrot a :Policy .

:Policy_Sermon a :Policy .

:Policy_Stick a :Policy .

:Sovereignty a schema:Intangible ;
    rdfs:comment "the exercise of power by a state" ;
    skos:narrower :SovereigntyDeFacto,
        :SovereigntyDeJure,
        :SovereigntyWestphalian ;
    schema:seeAlso "https://en.wikipedia.org/wiki/Sovereignty" .

:Standard rdfs:subClassOf :Policy .

:Stephen_Harper a schema:Person ;
    rdfs:label "Stephen Harper" ;
    :holdsOffice :PrimeMinisterCanada22 ;
    schema:memberOf :Conservative_Canada2 .

:chairOf a owl:ObjectProperty ;
    rdfs:domain schema:organizationRole ;
    rdfs:range schema:organization .

:hasProblem a owl:ObjectProperty ;
    rdfs:label "has problem"@en ;
    rdfs:domain rdfs:Resource ;
    rdfs:range :Problem .

:heads a owl:ObjectProperty ;
    rdfs:domain schema:organizationRole ;
    rdfs:range schema:organization .

:holdsOffice a owl:ObjectProperty ;
    rdfs:domain schema:Person ;
    rdfs:range :organizationRole .

:isAffectedBy a owl:ObjectProperty ;
    rdfs:label "is affected by"@en ;
    rdfs:comment "Indicates that a resource is influenced or impacted by another resource." ;
    rdfs:domain rdfs:Resource .

:mandate a schema:Intangible ;
    schema:additionalClass :BranchMandate,
        :DeptAgencyMandate,
        :DivisionMandate,
        :ProgramMandate,
        :SectorMandate,
        :TeamMandate .

:primeMinisterialOrder a owl:DatatypeProperty ;
    rdfs:domain :PrimeMinister ;
    rdfs:range xsd:integer .

lawslois:Librarian_and_Archivist a skos:Concept ;
    skos:definition "the Librarian and Archivist of Canada appointed under subsection 5(1)."@en ;
    skos:inScheme lawslois:Libraries_Archives_Act ;
    skos:prefLabel "Librarian and Archivist"@en,
        "Version anglaise seulement"@fr .

lawslois:Minister a skos:Concept ;
    skos:definition "the member of the Queen’s Privy Council for Canada who is designated by the Governor in Council as the Minister for the purposes of this Act."@en ;
    skos:inScheme lawslois:Libraries_Archives_Act ;
    skos:prefLabel "Minister"@en,
        "ministre"@fr .

lawslois:documentary_heritage a skos:Concept ;
    skos:definition "publications and records of interest to Canada."@en ;
    skos:inScheme lawslois:Libraries_Archives_Act ;
    skos:prefLabel "documentary heritage"@en,
        "patrimoine documentaire"@fr .

lawslois:government_institution a skos:Concept ;
    skos:definition "an institution designated by the Governor in Council."@en ;
    skos:inScheme lawslois:Libraries_Archives_Act ;
    skos:prefLabel "government institution"@en,
        "institution fédérale"@fr .

lawslois:government_record a skos:Concept ;
    skos:definition "a record that is under the control of a government institution."@en ;
    skos:inScheme lawslois:Libraries_Archives_Act ;
    skos:prefLabel "government record"@en,
        "document fédéral"@fr .

lawslois:ministerial_record a skos:Concept ;
    skos:definition "a record of a member of the Queen’s Privy Council for Canada who holds the office of a minister and that pertains to that office, other than a record that is of a personal or political nature or that is a government record."@en ;
    skos:inScheme lawslois:Libraries_Archives_Act ;
    skos:prefLabel "ministerial record"@en,
        "document ministériel"@fr .

lawslois:publication a skos:Concept ;
    skos:definition "any library matter that is made available in multiple copies or at multiple locations, whether without charge or otherwise, to the public generally or to qualifying members of the public by subscription or otherwise. Publications may be made available through any medium and may be in any form, including printed material, on-line items or recordings."@en ;
    skos:inScheme lawslois:Libraries_Archives_Act ;
    skos:prefLabel "publication"@en,
        "publication"@fr .

lawslois:record a skos:Concept ;
    skos:definition "any documentary material other than a publication, regardless of medium or form."@en ;
    skos:inScheme lawslois:Libraries_Archives_Act ;
    skos:prefLabel "record"@en,
        "document"@fr .

schema:Legislation a schema:CreativeWork .

gc:DataGovernance a gc:Governance .

gc:DelegatedAuthority schema:isPartOf gc:CrownAuthority .

gc:EXPublicServant a gc:PublicServant ;
    rdfs:comment "significant executive managerial roles and responsibilities, significant executive policy roles and responsibilities, or significant influence on the direction of a department or agency" ;
    schema:memberOf gc:PublicServant ;
    schema:subjectOf gc:EXJobStandard2022 .

gc:GlossaryDS23 a skos:ConceptScheme ;
    rdfs:label "Data Strategy for the Federal Public Service - Annexes" ;
    schema:subject :DataAndInfo ;
    schema:url "https://wiki.gccollab.ca/Data_Strategy_for_the_Federal_Public_Service_-_Annexes" .

gc:GuidanceDataQuality a schema:CreativeWork ;
    rdfs:label "Guidance on Data Quality" ;
    schema:subject :DataQuality ;
    schema:url "https://www.canada.ca/en/government/system/digital-government/digital-government-innovations/information-management/guidance-assessing-readiness-manage-data-according-findable-accessible-interoperable-reusable-principles.html" .

gc:GuidanceMetadataNeeds a schema:CreativeWork ;
    rdfs:label "Guidance on Assessing Metadata Needs" ;
    schema:subject :Metadata ;
    schema:url "https://www.canada.ca/en/government/system/digital-government/digital-government-innovations/information-management/guidance-assessing-metadata-needs.html" .

gc:administrative_decision a skos:Concept ;
    skos:definition "Any  decision that is made by an authorized official of a department as  identified in section 8 of this directive pursuant to powers conferred by an Act of Parliament or an order made pursuant to a prerogative of  the Crown that affects legal rights, privileges or interests."@en,
        "Toute décision prise par une personne autorisée  d’un ministère, visée à la section 8 de la Directive, en application des  pouvoirs que lui confère une loi du Parlement ou une ordonnance prise en vertu  de la prérogative de la Couronne et qui touche des droits juridiques, les  privilèges ou les intérêts d’une personne."@fr ;
    skos:inScheme gc:DIRECTIVE_automateddecisionmaking ;
    skos:prefLabel "administrative  decision"@en,
        "Décision administrative"@fr .

gc:algorithmic_impact_assessment a skos:Concept ;
    skos:definition "A framework  to help  departments better  understand and reduce the risks associated with automated decision systems and  to provide the appropriate  requirements that best match the  type of  system being designed."@en,
        "Cadre destiné à aider ministères à mieux comprendre les risques associés aux systèmes décisionnels automatisés, à les  atténuer et à définir les exigences appropriées qui correspondent le mieux au  type de système conçu."@fr ;
    skos:inScheme gc:DIRECTIVE_automateddecisionmaking ;
    skos:prefLabel "algorithmic impact assessment"@en,
        "Évaluation de l’incidence algorithmique"@fr .

gc:automated_decision_system a skos:Concept ;
    skos:definition "Any  technology that either assists or replaces the judgment of human decision  makers. These systems draw from fields like statistics, linguistics and computer  science, and use techniques such as rules-based systems, regression, predictive  analytics, machine learning, deep learning, and neural networks."@en,
        "Toute technologie qui se substitue au  jugement des décideurs ou qui les assiste. Ces systèmes proviennent de domaines  tels ceux des statistiques, de la linguistique et de l’informatique. Ils  utilisent des techniques telles que les systèmes basés sur des règles, la  régression, l’analytique prédictive, l’apprentissage automatique,  l’apprentissage en profondeur et les réseaux neuronaux."@fr ;
    skos:inScheme gc:DIRECTIVE_automateddecisionmaking ;
    skos:prefLabel "automated decision system"@en,
        "Système décisionnel automatisé"@fr .

gc:gc-enterprise-data-reference-standards a schema:WebPage ;
    rdfs:label "Inventory of data and metadata reference standards"@en,
        "Liste des normes référentielles relatives aux données et aux métadonnées"@fr ;
    rdfs:seeAlso "https://www.canada.ca/en/government/system/digital-government/digital-government-innovations/enabling-interoperability/gc-enterprise-data-reference-standards.html"@en,
        "https://www.canada.ca/fr/gouvernement/systeme/gouvernement-numerique/innovations-gouvernementales-numeriques/permettre-interoperabilite/normes-referentielles-pangouvernementales-relatives-donnees-gc.html"@fr .

gc:human_rights a skos:Concept ;
    rdfs:seeAlso "https://www.canada.ca/en/canadian-heritage/services/about-human-rights.html"@en,
        "https://www.canada.ca/fr/patrimoine-canadien/services/a-propos-droits-personne.html"@fr ;
    skos:definition "The rights to which persons are inherently entitled because they are human beings (Source).  Human rights are protected in the Canadian Charter of Rights and Freedoms, Canadian Human Rights Act, and the United Nations Declaration on the Rights of Indigenous Peoples Act."@en ;
    skos:inScheme gc:DIRECTIVE_automateddecisionmaking ;
    skos:prefLabel "human rights"@en,
        "Droits de la personne"@fr .

gc:production a skos:Concept ;
    skos:definition "An automated decision system is in production when it is in use and has impacts on real clients. This can include when it is in beta or user testing and producing outputs that impact clients."@en,
        "Se dit d’un système décisionnel automatisé  qui est utilisé et qui a une incidence sur la clientèle réelle. Il peut s’agir d’un système en version bêta ou d’un système testé par les personnes qui l’utilisent, qui produit des résultats ayant une incidence sur la clientèle."@fr ;
    skos:inScheme gc:DIRECTIVE_automateddecisionmaking ;
    skos:prefLabel "production"@en,
        "En production"@fr .

gc:proprietary a skos:Concept ;
    skos:definition "Refers to  systems, algorithms or software owned by an entity, such as a company or government. These systems are often closed  source, meaning the source code is not publicly available."@en,
        "Se dit des systèmes, des algorithmes ou des  logiciels qui appartiennent à une entité, telle qu’une entreprise ou une  administration publique. Il s’agit souvent de systèmes à code fermé,  c’est-à-dire que le code source n’est pas accessible au public."@fr ;
    skos:inScheme gc:DIRECTIVE_automateddecisionmaking ;
    skos:prefLabel "proprietary"@en,
        "Propriétaire"@fr .

gc:test_environment a skos:Concept ;
    skos:definition "An environment containing hardware, instrumentation, simulators, software tools, and other support elements needed to conduct a test. A system in a test environment may mimic a production  environment but does not impact real clients. Test environments may include exploration zones and sandboxes."@en,
        "Environnement contenant du matériel, des instruments, des simulateurs, des outils logiciels et d’autres composantes nécessaires à la réalisation d’un essai. Le déploiement d’un système dans un environnement d’essai permet de simuler son fonctionnement dans un  environnement de production sans incidence sur la clientèle réelle. Il peut s’agir de zones d’exploration ou de bacs à sable."@fr ;
    skos:inScheme gc:DIRECTIVE_automateddecisionmaking ;
    skos:prefLabel "test  environment"@en,
        "Environnement d’essai"@fr .

wiki:Berlin_Wall a schema:LandmarksOrHistoricalBuildings ;
    schema:location wiki:Berlin .

wiki:Global_debt a skos:Concept .

wiki:Polity a skos:Concept,
        schema:AdministrativeArea ;
    rdfs:comment "a group of people with a collective identity, who are organized by some form of political institutionalized social relations, and have a capacity to mobilize resources" .

wiki:Polycrisis a schema:Intangible ;
    rdfs:label "polycrise"@fr ;
    rdfs:comment "complex situation where multiple, interconnected crises converge and amplify each other, resulting in a predicament that is difficult to manage or resolve." ;
    :includes wiki:Artificial_Intelligence,
        wiki:Climate_Change,
        wiki:Democratic_Backsliding,
        wiki:Global_debt,
        wiki:Inflation,
        wiki:Resource_Depletion,
        wiki:Social_Inequality,
        wiki:Synthetic_Biology,
        wiki:War,
        :COVID19Pandemic .

wiki:State a wiki:Polity .

:Asset a schema:Thing ;
    rdfs:comment "any resource owned or controlled by a business or an economic entity" ;
    schema:subjectOf "https://en.wikipedia.org/wiki/Asset" .

:COVID19Pandemic a schema:event ;
    schema:subjectOf "https://en.wikipedia.org/wiki/COVID-19_pandemic" .

:Canada a wiki:State,
        schema:Country ;
    rdfs:seeAlso "https://www.canada.ca/" ;
    schema:additionalProperty :SovereigntyCanadian ;
    schema:containedInPlace :NorthAmerica ;
    schema:memberOf :G7,
        :UnitedNations,
        :WorldTradeOrganization .

:Canadian a schema:Person ;
    schema:Nationality :Canada .

:Directive rdfs:subClassOf :Policy .

:Earth a schema:Place ;
    rdfs:label "World" ;
    schema:identifier "https://en.wikipedia.org/wiki/Earth" .

:GlobalTradeSystem a skos:Concept,
        schema:Intangible ;
    rdfs:comment "https://www.wto.org/english/thewto_e/whatis_e/tif_e/fact2_e.htm" ;
    :governedBy :WorldTradeOrganization .

:Governance a schema:OrganizeAction ;
    rdfs:comment "Governance establishes how the government exercises authority, accountability, leadership, direction and control" ;
    schema:subjectOf "https://www.canada.ca/en/government/system/digital-government/guideline-service-digital.html#ToC1" .

:InternationalOrganization a schema:organization .

:KingPrivyCouncilCanada a schema:GovernmentOrganization ;
    skos:prefLabel "King's Privy Council"@en ;
    schema:subOrganization :GovernmentCanada .

:Liberal_Unionist_Canada a schema:PoliticalParty ;
    :precededBy :Liberal_Canada ;
    :succeededBy :Liberal_Canada,
        :Unionist_Canada ;
    schema:dissolutionDate 1917 ;
    schema:foundingDate 1917 .

:Mark_Carney a schema:Person ;
    rdfs:label "Mark Carney" ;
    :holdsOffice :PrimeMinisterCanada24 ;
    schema:memberOf :Liberal_Canada .

:MinistryCanada1 a :MinistryCanada .

:MinistryCanada28 a :MinistryCanada .

:MinistryCanada29 a :MinistryCanada .

:MinistryCanada3 a :MinistryCanada .

:MinistryCanada30 a :MinistryCanada ;
    :hasResponsibility :Governance,
        :Priorities2025 ;
    schema:instrument "focus, determination, and fundamentally different approaches to governing" .

:NorthAmerica a schema:Continent ;
    skos:altLabel "Turtle Island" ;
    schema:containedInPlace :Earth .

:PrimeMinisterCanada1 a :PrimeMinisterCanada ;
    :chairOf :MinistryCanada1,
        :MinistryCanada3 ;
    :primeMinisterialOrder 1 .

:PrimeMinisterCanada22 a :PrimeMinisterCanada ;
    rdfs:label "The 22nd Prime Minister of Canada" ;
    :chairOf :MinistryCanada28 ;
    :primeMinisterialOrder 22 .

:PrimeMinisterCanada23 a :PrimeMinisterCanada ;
    rdfs:label "The 23rd Prime Minister of Canada" ;
    :chairOf :MinistryCanada29 ;
    :primeMinisterialOrder 23 .

:PrimeMinisterCanada24 a :PrimeMinisterCanada ;
    rdfs:label "The 24th Prime Minister of Canada" ;
    :chairOf :MinistryCanada30 ;
    :primeMinisterialOrder 24 .

:Progressive_Conservative_Canada a schema:PoliticalParty ;
    :succeededBy :Conservative_Canada2 ;
    schema:dissolutionDate 2003 ;
    schema:foundingDate 1942 .

:Results a schema:Intangible ;
    schema:subjectOf :DepartmentalResultsReport .

:RisingGeopoliticalRisk a :Problem ;
    rdfs:label "Rising Geopolitical Risk"@en .

:SovereigntyCanadian a :SovereigntyWestphalian ;
    schema:additionalType :SovereigntyDeFacto,
        :SovereigntyDeJure .

:SovietUnionCollapse a schema:event .

:Unionist_Canada a schema:PoliticalParty ;
    :precededBy :Conservative_Canada1,
        :Liberal_Unionist_Canada ;
    :succeededBy :Conservative_Canada1 ;
    schema:dissolutionDate 1922 ;
    schema:foundingDate 1917 .

:UnitedNations a :InternationalOrganization ;
    schema:identifier "https://www.un.org/en/" .

schema:AdministrativeArea a schema:Place .

schema:InternationalOrganization a schema:organization .

schema:WebPage a schema:CreativeWork .

gc:DeputyHead a schema:organizationRole ;
    rdfs:subClassOf gc:PublicServant ;
    :heads gc:DepartmentsAgencies ;
    schema:agent gc:DeliverMandate .

gc:EAframework a schema:CreativeWork ;
    rdfs:label "Government of Canada Enterprise Architecture Framework" ;
    schema:subject :EnterpriseArchitecture ;
    schema:url "https://www.canada.ca/en/government/system/digital-government/policies-standards/government-canada-enterprise-architecture-framework.html" .

gc:EXJobStandard2022 a schema:CreativeWork ;
    rdfs:label "Executive (EX) Group Job Evaluation Standard 2022" ;
    schema:url "https://www.canada.ca/en/treasury-board-secretariat/services/collective-agreements/job-evaluation/executive-group-position-evaluation-plan-2022.html" .

gc:FederalPublicService a schema:GovernmentOrganization .

gc:ServiceDigitalDefs a skos:ConceptScheme ;
    schema:url "https://www.tbs-sct.canada.ca/pol/doc-eng.aspx?id=32603#appA" .

:CanadianContext2025 a :hasContext ;
    :hasProblem :GlobalTradeSystemTransformation,
        :SovereigntyCanadianThreatened,
        :affordabilityCrisis,
        :longStandingLowProductivity,
        :strainedGovernmentFinances,
        :unsustainableSocialPrograms ;
    :isAffectedBy :GlobalContext2025 .

:Conservative_Canada2 a schema:PoliticalParty ;
    rdfs:label "Conservative Party of Canada"@en,
        "Parti conservateur du Canada"@fr ;
    schema:foundingDate 2003 .

:DataAndInfo a :Asset .

:EnterpriseArchitecture schema:subjectOf gc:EAframework .

:GlobalContext2025 a :hasContext ;
    :hasProblem wiki:Polycrisis,
        :RisingGeopoliticalRisk ;
    :isAffectedBy :danger,
        :division .

:Liberal_Conservative_Canada a schema:organization ;
    :succeededBy :Conservative_Canada1 ;
    schema:dissolutionDate 1938 ;
    schema:foundingDate 1867 ;
    schema:subjectOf "https://en.wikipedia.org/wiki/Liberal-Conservative_Party" .

:MandateLetter a schema:HowTo ;
    rdfs:label "Mandate Letter"@en,
        "Lettre de mandat"@fr ;
    rdfs:comment "a letter from Prime Minister to The Ministry outlining government committements and priorities." ;
    schema:about :Priorities ;
    schema:author :PrimeMinisterCanada .

:PrimeMinister a skos:Concept ;
    rdfs:subClassOf schema:organizationRole .

:Priorities2025 a :hasContext ;
    rdfs:label "Government Priorities 2025" ;
    :addresses :CanadianContext2025 ;
    schema:isPartOf :DeliverResultsForCanadians .

:SovereigntyDeFacto a schema:Intangible ;
    rdfs:comment "the factual ability to exercise sovereignty" ;
    schema:identifier "https://en.wikipedia.org/wiki/De_facto" .

:SovereigntyDeJure a schema:Intangible ;
    rdfs:comment "the legal right to exercise sovereignty" ;
    schema:identifier "https://en.wikipedia.org/wiki/De_jure" .

:SovereigntyWestphalian a schema:Intangible ;
    rdfs:comment "each state has exclusive sovereignty over its territory." ;
    schema:identifier "https://en.wikipedia.org/wiki/Westphalian_system" .

:WorldTradeOrganization a schema:InternationalOrganization ;
    rdfs:comment "the only international organization dealing with the rules of trade between nations." ;
    owl:ID "https://www.wto.org/" ;
    schema:administrativeArea :GlobalTradeSystem .

schema:Place a schema:Thing .

gc:DepartmentsAgencies a schema:GovernmentOrganization .

:Conservative_Canada1 a schema:PoliticalParty ;
    :succeededBy :Progressive_Conservative_Canada ;
    schema:dissolutionDate 1942 ;
    schema:foundingDate 1867 .

:DeliverResultsForCanadians a :DeliverMandate,
        schema:OrganizeAction ;
    schema:actionProcess :MandateLetter ;
    schema:agent :MinistryCanada ;
    schema:audience :Canadian ;
    schema:instrument :Policy ;
    schema:provider gc:DepartmentsAgencies ;
    schema:result :Results .

:Liberal_Canada a schema:PoliticalParty ;
    rdfs:label "Liberal Party of Canada"@en,
        "Parti liberal du Canada"@fr ;
    schema:foundingDate 1867 .

schema:GovernmentOrganization a schema:organization .

gc:PublicServant a schema:Employee ;
    schema:memberOf gc:FederalPublicService .

:PrimeMinisterCanada a skos:Concept ;
    rdfs:label "Prime Minister of Canada"@en,
        "Premier ministre du Canada"@fr ;
    rdfs:subClassOf :PrimeMinister .

:hasContext a owl:ObjectProperty ;
    rdfs:label "has context"@en ;
    rdfs:comment "A general background condition or situation that influences or frames a resource." .

:MinistryCanada a schema:GovernmentOrganization ;
    skos:altLabel "Cabinet"@en,
        "le Cabinet"@fr ;
    skos:prefLabel "Canadian Ministry"@en,
        "Le Conseil des ministres"@fr ;
    schema:subOrganization :KingPrivyCouncilCanada .

schema:CreativeWork a schema:Thing .

schema:Person a schema:Thing .

schema:Thing a owl:Thing .

schema:organization a schema:Thing .

gc:DIRECTIVE_automateddecisionmaking a skos:ConceptScheme,
        :Directive ;
    rdfs:label "Directive on Automated Decision Making"@en,
        "Directive sur la prise de décisions automatisée"@fr ;
    dcterms:modified "2017-08-24" ;
    rdfs:seeAlso "https://www.tbs-sct.canada.ca/pol/doc-eng.aspx?id=DIRECTIVE_automateddecisionmaking" .

lawslois:Libraries_Archives_Act a schema1:Legislation,
        skos:ConceptScheme ;
    rdfs:label "Definitions from l-7.7 Act"@en ;
    rdfs:seeAlso "https://laws-lois.justice.gc.ca/eng/acts/l-7.7/"@en,
        "https://laws-lois.justice.gc.ca/fra/lois/l-7.7/"@fr .

schema:Intangible a schema:Thing .

