PREFIX :<>
PREFIX schema:<http://www.schema.org/>
PREFIX wiki:<https://en.wikipedia.org/wiki/>
PREFIX cst:<https://canada.multites.net/cst/#>
PREFIX rdfs:<http://www.w3.org/2000/01/rdf-schema#> 
PREFIX xsd: <http://www.w3.org/2001/XMLSchema#> 
PREFIX gc:<https://www.canada.ca/#>
PREFIX skos: <http://www.w3.org/2004/02/skos/core#> 

gc:ServiceDigitalDefs1 a skos:Concept ;
    skos:prefLabel "Applications"@en , "Applications"@fr ;
    skos:definition "Subclass of software that employs the capabilities of an electronic device directly and thoroughly for a task that the user wishes to perform."@en ;
    skos:inScheme gc:ServiceDigitalDefs ;
    :subject cst:1718
    .

gc:ServiceDigitalDefs2 a skos:Concept ;
    skos:prefLabel "Artificial Intelligence"@en , "Intelligence artificielle"@fr ;
    skos:definition "Information technology that performs tasks that would ordinarily require biological brainpower to accomplish, such as making sense of spoken language, learning behaviours, or solving problems."@en ;
    skos:inScheme gc:ServiceDigitalDefs ;
    :subject cst:767
    .

gc:ServiceDigitalDefs3 a skos:Concept ;
    skos:prefLabel "Automated Decision System"@en , "Système décisionnel automatisé"@fr ;
    skos:definition "Includes any technology that either assists or replaces the judgement of human decision-makers. These systems draw from fields like statistics, linguistics, and computer science, and use techniques such as rules-based systems, regression, predictive analytics, machine learning, deep learning, and neural nets."@en ;
    skos:inScheme gc:ServiceDigitalDefs ;
    :subject cst:884
    .

gc:ServiceDigitalDefs4 a skos:Concept ;
    skos:prefLabel "Client"@en , "Client"@fr ;
    skos:definition "Individuals, businesses or their representatives served by or using either internal or external services provided by the Government of Canada. When describing interactions with information technologies, clients can be referred to as users."@en ;
    skos:inScheme gc:ServiceDigitalDefs
    .

gc:ServiceDigitalDefs5 a skos:Concept ;
    skos:prefLabel "Client-centric"@en , "Axé sur les clients"@fr ;
    skos:definition "An approach that focuses on addressing client or user expectations, needs, challenges and feedback. It enables the creation of a positive experience for the client or user, considering a broad range of factors such as access, inclusion, accessibility, security, privacy, simplicity, and choice of official language."@en ;
    skos:inScheme gc:ServiceDigitalDefs
    .

gc:ServiceDigitalDefs6 a skos:Concept ;
    skos:prefLabel "Client feedback"@en, "Rétroaction du client"@fr ;
    skos:definition "Information coming directly from recipients of services about the satisfaction or dissatisfaction they feel with a service or product, and is a critical part of service improvement. It can take several forms, including: in-service client feedback, client satisfaction surveys, user experience testing, and consultations."@en ;
    skos:inScheme gc:ServiceDigitalDefs
    .

gc:ServiceDigitalDefs7 a skos:Concept ;
    skos:prefLabel "COBIT"@en , "COBIT"@fr ;
    skos:definition "Stands for 'Control Objectives for Information and related Technology' and represents a set of best practices that provide guidance for the management of IT processes. (Source: IT Governance Institute)"@en ;
    skos:inScheme gc:ServiceDigitalDefs
    .

gc:ServiceDigitalDefs8 a skos:Concept ;
    skos:prefLabel "Cyber security"@en , "Cybersécurité"@fr ;
    skos:definition "The body of technologies, processes, practices and response and mitigation measures designed to protect electronic information and information infrastructure from mischief, unauthorized use, or disruption."@en ;
    skos:inScheme gc:ServiceDigitalDefs
    .

gc:ServiceDigitalDefs9 a skos:Concept ;
    skos:prefLabel "Data"@en , "Données"@fr ;
    skos:definition "Set of values of subjects with respect to qualitative or quantitative variables representing facts, statistics, or items of information in a formalized manner suitable for communication, reinterpretation, or processing."@en ;
    skos:inScheme gc:ServiceDigitalDefs
    .

gc:ServiceDigitalDefs10 a skos:Concept ;
    skos:prefLabel "Devices"@en , "Dispositifs"@fr ;
    skos:definition "Electronic tools that can include, but are not limited to, the following: desktop workstations, laptops, notebooks, tablets, cellphones, peripherals such as printers and scanners, memory drives, CD/DVD drives, webcams and any other hardware used to obtain, store, or send information."@en ;
    skos:inScheme gc:ServiceDigitalDefs
    .

gc:ServiceDigitalDefs11 a skos:Concept ;
    skos:prefLabel "Digital"@en , "Numérique"@fr ;
    skos:definition "Processes, practices and technologies related to the production, storage, processing, dissemination and exchange of electronic information and data.  It refers to, among other things, information and communications technologies, infrastructures, and the information and data they produce and collect."@en ;
    skos:inScheme gc:ServiceDigitalDefs
    .
