PREFIX :<>
PREFIX schema:<http://www.schema.org/>
PREFIX wiki:<https://en.wikipedia.org/wiki/>
PREFIX cst:<http://www.thesaurus.gc.ca/#>
PREFIX rdfs:<http://www.w3.org/2000/01/rdf-schema#> 
PREFIX gc:<https://www.canada.ca/#>
PREFIX skos:<http://www.w3.org/2004/02/skos/core#> 
PREFIX lawslois:<https://laws-lois.justice.gc.ca/eng/acts/>
PREFIX dcterms:<http://purl.org/dc/terms/>

gc:MDRS a schema:CreativeWork ;
    rdfs:label "Operational Standard for Digital Archival Records’ Metadata" ;
    schema:identifier "https://library-archives.canada.ca/eng/services/government-canada/information-disposition/managing-government-records/guidelines-information-management/Pages/operational-standard-digital-archival-records-metadata.aspx" ;
    :authorizedBy :LAC_GovtRecordDG
    .

# Library and Archives Act & definitions
lawslois:L_7_7 a skos:ConceptScheme ;
  rdfs:label "Library and Archives Act"@en , "Loi sur la Bibliothèque et les Archives du Canada"@fr ;
  rdfs:seeAlso "https://laws-lois.justice.gc.ca/eng/acts/l-7.7/"@en , "https://laws-lois.justice.gc.ca/fra/lois/l-7.7/"@fr ;
.

lawslois:documentary_heritage a skos:Concept ;
  skos:prefLabel "documentary heritage"@en  , "patrimoine documentaire"@fr ;
  skos:definition "publications and records of interest to Canada."@en ;
  skos:inScheme lawslois:L_7_7 ;
.

lawslois:government_institution a skos:Concept ;
  skos:prefLabel "government institution"@en  , "institution fédérale"@fr ;
  skos:definition "an institution designated by the Governor in Council."@en ;
  skos:inScheme lawslois:L_7_7 ;
.

lawslois:government_record a skos:Concept ;
  skos:prefLabel "government record"@en  , "document fédéral"@fr ;
  skos:definition "a record that is under the control of a government institution."@en ;
  skos:inScheme lawslois:L_7_7 ;
.

lawslois:Librarian_and_Archivist a skos:Concept ;
  skos:prefLabel "Librarian and Archivist"@en  , "Version anglaise seulement"@fr ;
  skos:definition "the Librarian and Archivist of Canada appointed under subsection 5(1)."@en ;
  skos:inScheme lawslois:L_7_7 ;
.

lawslois:Minister a skos:Concept ;
  skos:prefLabel "Minister"@en  , "ministre"@fr ;
  skos:definition "the member of the Queen’s Privy Council for Canada who is designated by the Governor in Council as the Minister for the purposes of this Act."@en ;
  skos:inScheme lawslois:L_7_7 ;
.

lawslois:ministerial_record a skos:Concept ;
  skos:prefLabel "ministerial record"@en  , "document ministériel"@fr ;
  skos:definition "a record of a member of the Queen’s Privy Council for Canada who holds the office of a minister and that pertains to that office, other than a record that is of a personal or political nature or that is a government record."@en ;
  skos:inScheme lawslois:L_7_7 ;
  skos:broader cst:records
.

lawslois:publication a skos:Concept ;
  skos:prefLabel "publication"@en  , "publication"@fr ;
  skos:definition "any library matter that is made available in multiple copies or at multiple locations, whether without charge or otherwise, to the public generally or to qualifying members of the public by subscription or otherwise. Publications may be made available through any medium and may be in any form, including printed material, on-line items or recordings."@en ;
  skos:inScheme lawslois:L_7_7 ;
.

lawslois:record a skos:Concept ;
  skos:prefLabel "record"@en  , "document"@fr ;
  skos:definition "any documentary material other than a publication, regardless of medium or form."@en ;
  skos:inScheme lawslois:L_7_7 ;
.

# Privacy Act & definitions

lawslois:P21 a skos:ConceptScheme ;
  rdfs:label "Definitions from P-21 Act"@en ;
  rdfs:seeAlso "https://laws-lois.justice.gc.ca/eng/acts/P-21/" ;
.

lawslois:administrative_purpose a skos:Concept ;
  skos:prefLabel "administrative purpose"@en  , "fins administratives"@fr ;
  skos:definition "the use of that information in a decision making process that directly affects that individual;"@en ;
  skos:inScheme lawslois:P21 ;
.

lawslois:alternative_format a skos:Concept ;
  skos:prefLabel "alternative format"@en  , "support de substitution"@fr ;
  skos:definition "a format that allows a person with a sensory disability to read or listen to the personal information;"@en ;
  skos:inScheme lawslois:P21 ;
.

lawslois:Court a skos:Concept ;
  skos:prefLabel "Court"@en  , "Cour"@fr ;
  skos:definition "the Federal Court;"@en ;
  skos:inScheme lawslois:P21 ;
.

lawslois:designated_Minister a skos:Concept ;
  skos:prefLabel "designated Minister"@en  , "ministre désigné"@fr ;
  skos:definition "a person who is designated as the Minister under subsection 3.1(1);"@en ;
  skos:inScheme lawslois:P21 ;
.

lawslois:government_institution a skos:Concept ;
  skos:prefLabel "government institution"@en  , "institution fédérale"@fr ;
  skos:definition "(a)any department or ministry of state of the Government of Canada, or any body or office, listed in the schedule, and(b)any parent Crown corporation, and any wholly-owned subsidiary of such a corporation, within the meaning of section 83 of theFinancial Administration Act;"@en ;
  skos:inScheme lawslois:P21 ;
.

lawslois:head a skos:Concept ;
  skos:prefLabel "head"@en  , "responsable d’institution fédérale"@fr ;
  skos:definition "(a)in the case of a department or ministry of state, the member of the Queen’s Privy Council for Canada who presides over the department or ministry, or(b)in any other case, either the person designated under subsection 3.1(2) to be the head of the institution for the purposes of this Act or, if no such person is designated, the chief executive officer of the institution, whatever their title;"@en ;
  skos:inScheme lawslois:P21 ;
.

lawslois:personal_information a skos:Concept ;
  skos:prefLabel "personal information"@en  , "renseignements personnels"@fr ;
  skos:definition "information about an identifiable individual that is recorded in any form including, without restricting the generality of the foregoing,(a)information relating to the race, national or ethnic origin, colour, religion, age or marital status of the individual,(b)information relating to the education or the medical, criminal or employment history of the individual or information relating to financial transactions in which the individual has been involved,(c)any identifying number, symbol or other particular assigned to the individual,(d)the address, fingerprints or blood type of the individual,(e)the personal opinions or views of the individual except where they are about another individual or about a proposal for a grant, an award or a prize to be made to another individual by a government institution or a part of a government institution specified in the regulations,(f)correspondence sent to a government institution by the individual that is implicitly or explicitly of a private or confidential nature, and replies to such correspondence that would reveal the contents of the original correspondence,(g)the views or opinions of another individual about the individual,(h)the views or opinions of another individual about a proposal for a grant, an award or a prize to be made to the individual by an institution or a part of an institution referred to in paragraph (e), but excluding the name of the other individual where it appears with the views or opinions of the other individual, and(i)the name of the individual where it appears with other personal information relating to the individual or where the disclosure of the name itself would reveal information about the individual,but, for the purposes of sections 7, 8 and 26 and section 19 of theAccess to Information Act, does not include(j)information about an individual who is or was an officer or employee of a government institution that relates to the position or functions of the individual including,(i)the fact that the individual is or was an officer or employee of the government institution,(ii)the title, business address and telephone number of the individual,(iii)the classification, salary range and responsibilities of the position held by the individual,(iv)the name of the individual on a document prepared by the individual in the course of employment, and(v)the personal opinions or views of the individual given in the course of employment,(j.1)the fact that an individual is or was aministerial adviseror a member of aministerial staff, as those terms are defined in subsection 2(1) of theConflict of Interest Act, as well as the individual’s name and title,(k)information about an individual who is or was performing services under contract for a government institution that relates to the services performed, including the terms of the contract, the name of the individual and the opinions or views of the individual given in the course of the performance of those services,(l)information relating to any discretionary benefit of a financial nature, including the granting of a licence or permit, conferred on an individual, including the name of the individual and the exact nature of the benefit, and(m)information about an individual who has been dead for more than twenty years;"@en ;
  skos:inScheme lawslois:P21 ;
.

lawslois:personal_information_bank a skos:Concept ;
  skos:prefLabel "personal information bank"@en  , "fichier de renseignements personnels"@fr ;
  skos:definition "a collection or grouping of personal information described in section 10;"@en ;
  skos:inScheme lawslois:P21 ;
.

lawslois:Privacy_Commissioner a skos:Concept ;
  skos:prefLabel "Privacy Commissioner"@en  , "Commissaire à la protection de la vie privée"@fr ;
  skos:definition "the Commissioner appointed under section 53;"@en ;
  skos:inScheme lawslois:P21 ;
.

lawslois:sensory_disability a skos:Concept ;
  skos:prefLabel "sensory disability"@en  , "déficience sensorielle"@fr ;
  skos:definition "a disability that relates to sight or hearing."@en ;
  skos:inScheme lawslois:P21 ;
.

# Directive on Automated Decision Making Definitions

tbspol:32592 a skos:ConceptScheme ;
  rdfs:label "Directive on Automated Decision Making"@en , "Directive sur la prise de décisions automatisée"@fr;
  rdfs:seeAlso "https://www.tbs-sct.canada.ca/pol/doc-eng.aspx?id=32592" ;
  dcterms:modified "2017-08-24".

tbspol:administrative_decision a skos:Concept ;
  skos:prefLabel "administrative  decision"@en , "Décision administrative"@fr;
  skos:definition "Any  decision that is made by an authorized official of a department as  identified in section 8 of this directive pursuant to powers conferred by an Act of Parliament or an order made pursuant to a prerogative of  the Crown that affects legal rights, privileges or interests."@en , "Toute décision prise par une personne autorisée  d’un ministère, visée à la section 8 de la Directive, en application des  pouvoirs que lui confère une loi du Parlement ou une ordonnance prise en vertu  de la prérogative de la Couronne et qui touche des droits juridiques, les  privilèges ou les intérêts d’une personne."@fr;
  skos:inScheme tbspol:32592 ;
.

tbspol:algorithmic_impact_assessment a skos:Concept ;
  skos:prefLabel "algorithmic impact assessment"@en , "Évaluation de l’incidence algorithmique"@fr ;
  skos:definition "A framework  to help  departments better  understand and reduce the risks associated with automated decision systems and  to provide the appropriate  requirements that best match the  type of  system being designed."@en , "Cadre destiné à aider ministères à mieux comprendre les risques associés aux systèmes décisionnels automatisés, à les  atténuer et à définir les exigences appropriées qui correspondent le mieux au  type de système conçu."@fr ;
  skos:inScheme tbspol:32592 ;
.

tbspol:automated_decision_system a skos:Concept ;
  skos:prefLabel "automated decision system"@en , "Système décisionnel automatisé"@fr;
  skos:definition "Any  technology that either assists or replaces the judgment of human decision  makers. These systems draw from fields like statistics, linguistics and computer  science, and use techniques such as rules-based systems, regression, predictive  analytics, machine learning, deep learning, and neural networks."@en , "Toute technologie qui se substitue au  jugement des décideurs ou qui les assiste. Ces systèmes proviennent de domaines  tels ceux des statistiques, de la linguistique et de l’informatique. Ils  utilisent des techniques telles que les systèmes basés sur des règles, la  régression, l’analytique prédictive, l’apprentissage automatique,  l’apprentissage en profondeur et les réseaux neuronaux."@fr ;
  skos:inScheme tbspol:32592 ;
  :subject cst:2074
.

tbspol:human_rights a skos:Concept ;
  skos:prefLabel "human rights"@en , "Droits de la personne"@fr;
  skos:definition "The rights to which persons are inherently entitled because they are human beings (Source).  Human rights are protected in the Canadian Charter of Rights and Freedoms, Canadian Human Rights Act, and the United Nations Declaration on the Rights of Indigenous Peoples Act."@en ;
  rdfs:seeAlso "https://www.canada.ca/en/canadian-heritage/services/about-human-rights.html"@en , "https://www.canada.ca/fr/patrimoine-canadien/services/a-propos-droits-personne.html"@fr ;
  skos:inScheme tbspol:32592 ;
.

tbspol:production a skos:Concept ;
  skos:prefLabel "production"@en , "En production"@fr;
  skos:definition "An automated decision system is in production when it is in use and has impacts on real clients. This can include when it is in beta or user testing and producing outputs that impact clients."@en , "Se dit d’un système décisionnel automatisé  qui est utilisé et qui a une incidence sur la clientèle réelle. Il peut s’agir d’un système en version bêta ou d’un système testé par les personnes qui l’utilisent, qui produit des résultats ayant une incidence sur la clientèle."@fr ;
  skos:inScheme tbspol:32592 ;
.

tbspol:proprietary a skos:Concept ;
  skos:prefLabel "proprietary"@en , "Propriétaire"@fr ;
  skos:definition "Refers to  systems, algorithms or software owned by an entity, such as a company or government. These systems are often closed  source, meaning the source code is not publicly available."@en , "Se dit des systèmes, des algorithmes ou des  logiciels qui appartiennent à une entité, telle qu’une entreprise ou une  administration publique. Il s’agit souvent de systèmes à code fermé,  c’est-à-dire que le code source n’est pas accessible au public."@fr ;
  skos:inScheme tbspol:32592 ;
.

tbspol:test_environment a skos:Concept ;
  skos:prefLabel "test  environment"@en , "Environnement d’essai"@fr;
  skos:definition "An environment containing hardware, instrumentation, simulators, software tools, and other support elements needed to conduct a test. A system in a test environment may mimic a production  environment but does not impact real clients. Test environments may include exploration zones and sandboxes."@en , "Environnement contenant du matériel, des instruments, des simulateurs, des outils logiciels et d’autres composantes nécessaires à la réalisation d’un essai. Le déploiement d’un système dans un environnement d’essai permet de simuler son fonctionnement dans un  environnement de production sans incidence sur la clientèle réelle. Il peut s’agir de zones d’exploration ou de bacs à sable."@fr ;
  skos:inScheme tbspol:32592 ;
.

